06GroupedEnvironments/GroupedEnvironments.thy
@@ -1,0 +1,344 @@
+theory GroupedEnvironments
+  imports "../02Typed/Type" "../00Utils/Environment" "../00Utils/Iteration"
+begin
+
+section \<open>Grouped Environments\<close>
+
+text \<open>We have now eliminated every expression-walking function in the evaluation process, but there 
+is still one recursive function, sort of: \<open>lookup\<close>. \<open>lookup\<close> is implemented as a recursive search 
+through a list, but fairly clearly it is equivalent to an indexed lookup which could be done in 
+constant time. So we don't have to worry about it.\<close>
+
+text \<open>Or do we? Looking ahead a bit, we will eventually need to represent our environments somehow 
+in a concrete machine: probably as contiguous arrays of pointers. This makes our \<open>lookup\<close> operation 
+as cheap as it should be, just an array access. But there is a problem: we don't only have one 
+environment. In a simpler block-structured language without function closures, we could use a single 
+stack as our environment, pushing and popping new bindings each time they go in and out of scope, 
+and accessing variables cheaply. But we have functions that close over their declaration 
+environment, and moreover these closures can be duplicated and applied multiple times - and thus 
+have their environments extended in different ways. Blindly copying the environments every time we 
+need a new closure keeps our lookups cheap, but means that every function application takes time
+linear in the size of the function closure's environment - an extremely unattractive prospect. 
+Alternately, we could keep representing environments by a linked list, which can have new bindings 
+cons'd onto the end cheaply and repeatedly, but means we _have to_ use the recursive list-search
+implementation of \<open>lookup\<close>, making every variable reference take time proportional to its Debruijn 
+index. Since any program is going to have many applications and variables, neither approach seems
+attractive.\<close>
+
+text \<open>Fortunately, there is a clever third option that combines many of the strengths of both 
+representations. Because we have let-floated our bindings, every let-binder is in a list of bindings 
+directly below a lambda-binder (or at the outside of the program at the top level). This means that 
+every time the lambda-abstraction is instantiated, all the let-bindings must also be instantiated; 
+so, without losing any sharing, we can allocate the environment for all the binders together in one 
+contiguous block. This permits the cheap pointer-copying environment-sharing of the second method 
+above, while reducing the cost of variable lookups to proportional to the number of enclosing 
+_functions_ rather than enclosing binders: since we know statically what frame and offset within 
+that frame a variable is defined at, we can follow pointers back to that frame and then look up the
+index directly. This key optimization makes the whole system adequately efficient, and is 
+more-or-less how real language implementations allocate environment memory*.\<close>
+
+text \<open>*We are slightly less efficient than real implementations because in practice most lambda 
+abstractions occur in blocks too, and a sequence of lambdas is usually instantiated all at once. 
+This allows for the further optimization of allocating environment frames for an entire block of 
+lambdas at once, producing a slight loss of sharing on curried applications in exchange for further 
+reducing lookup times to proportional to the number of enclosing lambda-_sequences_. Since most 
+functions are defined at the top level, this means that lookups are close to constant-time. See our 
+further work section.\<close>
+
+text \<open>We are not at the stage of actually representing environments in memory yet, of course. But by 
+the time we are, we will have compiled away much of the structure of the expressions, making it much 
+more difficult to calculate the frames-and-offsets from Debruijn indexes. So now, just before we 
+start compiling our expressions into linear code, we change our abstract environments from single 
+lists to lists-of-lists, representing the eventual linked-list-of-frames they will be, and replace 
+our variable indexes with frame-offset pairs. (We also precalculate and store the size of the frame 
+associated with a lambda-expression and store it for use later as well.)\<close>
+
+
+datatype expr\<^sub>g = 
+  Var\<^sub>g nat nat
+  | Const\<^sub>g nat
+  | Lam\<^sub>g ty expr\<^sub>g nat
+  | App\<^sub>g expr\<^sub>g expr\<^sub>g
+  | Let\<^sub>g expr\<^sub>g expr\<^sub>g
+
+text \<open>Typing remains almost unchanged, but we need to adjust the typing context a little: rather 
+than just a list, it too is a list of lists to match the new way we look up variables.\<close>
+
+fun let_count :: "expr\<^sub>g \<Rightarrow> nat" where
+  "let_count (Let\<^sub>g e\<^sub>1 e\<^sub>2) = Suc (let_count e\<^sub>2)"
+| "let_count e = 0"
+
+inductive typing\<^sub>g :: "ty list list \<Rightarrow> expr\<^sub>g \<Rightarrow> ty \<Rightarrow> bool" (infix "\<turnstile>\<^sub>g _ :" 50) where
+  tc\<^sub>g_var [simp]: "lookup \<Gamma> x = Some ts \<Longrightarrow> lookup ts y = Some t \<Longrightarrow> \<Gamma> \<turnstile>\<^sub>g Var\<^sub>g x y : t"
+| tc\<^sub>g_const [simp]: "\<Gamma> \<turnstile>\<^sub>g Const\<^sub>g n : Num"
+| tc\<^sub>g_lam [simp]: "insert_at 0 [t\<^sub>1] \<Gamma> \<turnstile>\<^sub>g e : t\<^sub>2 \<Longrightarrow> \<Gamma> \<turnstile>\<^sub>g Lam\<^sub>g t\<^sub>1 e (let_count e) : Arrow t\<^sub>1 t\<^sub>2"
+| tc\<^sub>g_app [simp]: "\<Gamma> \<turnstile>\<^sub>g e\<^sub>1 : Arrow t\<^sub>1 t\<^sub>2 \<Longrightarrow> \<Gamma> \<turnstile>\<^sub>g e\<^sub>2 : t\<^sub>1 \<Longrightarrow> \<Gamma> \<turnstile>\<^sub>g App\<^sub>g e\<^sub>1 e\<^sub>2 : t\<^sub>2"
+| tc\<^sub>g_let [simp]: "\<Gamma> \<turnstile>\<^sub>g e\<^sub>1 : t\<^sub>1 \<Longrightarrow> mapfst (insert_at 0 t\<^sub>1) \<Gamma> \<turnstile>\<^sub>g e\<^sub>2 : t\<^sub>2 \<Longrightarrow> \<Gamma> \<turnstile>\<^sub>g Let\<^sub>g e\<^sub>1 e\<^sub>2 : t\<^sub>2"
+
+inductive_cases [elim]: "\<Gamma> \<turnstile>\<^sub>g Var\<^sub>g x y : t"
+inductive_cases [elim]: "\<Gamma> \<turnstile>\<^sub>g Const\<^sub>g n : t"
+inductive_cases [elim]: "\<Gamma> \<turnstile>\<^sub>g Lam\<^sub>g t' e n : t"
+inductive_cases [elim]: "\<Gamma> \<turnstile>\<^sub>g App\<^sub>g e\<^sub>1 e\<^sub>2 : t"
+inductive_cases [elim]: "\<Gamma> \<turnstile>\<^sub>g Let\<^sub>g e\<^sub>1 e\<^sub>2 : t"
+
+text \<open>Closures, frames, and states need to be changed similarly.\<close>
+
+datatype closure\<^sub>g = 
+  Num\<^sub>g nat
+  | Fun\<^sub>g ty "closure\<^sub>g list list" expr\<^sub>g nat
+
+inductive typing_closure\<^sub>g :: "closure\<^sub>g \<Rightarrow> ty \<Rightarrow> bool" (infix ":\<^sub>g\<^sub>c\<^sub>l" 50)
+      and typing_environment\<^sub>g :: "closure\<^sub>g list list \<Rightarrow> ty list list \<Rightarrow> bool" (infix ":\<^sub>g\<^sub>c\<^sub>l\<^sub>s" 50) where
+  tc\<^sub>c_const [simp]: "Num\<^sub>g n :\<^sub>g\<^sub>c\<^sub>l Num"
+| tc\<^sub>c_lam [simp]: "\<Delta> :\<^sub>g\<^sub>c\<^sub>l\<^sub>s \<Gamma> \<Longrightarrow> insert_at 0 [t\<^sub>1] \<Gamma> \<turnstile>\<^sub>g e : t\<^sub>2 \<Longrightarrow> 
+    Fun\<^sub>g t\<^sub>1 \<Delta> e (let_count e) :\<^sub>g\<^sub>c\<^sub>l Arrow t\<^sub>1 t\<^sub>2"
+| tc\<^sub>c_nil [simp]: "[] :\<^sub>g\<^sub>c\<^sub>l\<^sub>s []"
+| tc\<^sub>c_cons_nil [simp]: "\<Delta> :\<^sub>g\<^sub>c\<^sub>l\<^sub>s \<Gamma> \<Longrightarrow> [] # \<Delta> :\<^sub>g\<^sub>c\<^sub>l\<^sub>s [] # \<Gamma>"
+| tc\<^sub>c_cons_cons [simp]: "c :\<^sub>g\<^sub>c\<^sub>l t \<Longrightarrow>  cs # \<Delta> :\<^sub>g\<^sub>c\<^sub>l\<^sub>s ts # \<Gamma> \<Longrightarrow> (c # cs) # \<Delta> :\<^sub>g\<^sub>c\<^sub>l\<^sub>s (t # ts) # \<Gamma>"
+
+inductive_cases [elim]:"Num\<^sub>g n :\<^sub>g\<^sub>c\<^sub>l t"
+inductive_cases [elim]: "Fun\<^sub>g t\<^sub>1 \<Delta> e n :\<^sub>g\<^sub>c\<^sub>l t"
+inductive_cases [elim]: "[] :\<^sub>g\<^sub>c\<^sub>l\<^sub>s \<Gamma>"
+inductive_cases [elim]: "[] # \<Delta> :\<^sub>g\<^sub>c\<^sub>l\<^sub>s \<Gamma>"
+inductive_cases [elim]: "(c # cs) # \<Delta> :\<^sub>g\<^sub>c\<^sub>l\<^sub>s \<Gamma>"
+
+lemma  "c :\<^sub>g\<^sub>c\<^sub>l t \<Longrightarrow> True"
+  and lookup_in_env\<^sub>g [simp]: "\<Delta> :\<^sub>g\<^sub>c\<^sub>l\<^sub>s \<Gamma> \<Longrightarrow> lookup \<Gamma> x = Some ts \<Longrightarrow> lookup ts y = Some t \<Longrightarrow>
+    \<exists>cs c. lookup \<Delta> x = Some cs \<and> lookup cs y = Some c \<and> c :\<^sub>g\<^sub>c\<^sub>l t"
+proof (induction c t and \<Delta> \<Gamma> arbitrary: and x ts y rule: typing_closure\<^sub>g_typing_environment\<^sub>g.inducts)
+  case (tc\<^sub>c_cons_nil \<Delta> \<Gamma>)
+  thus ?case by (cases x) simp_all
+next
+  case (tc\<^sub>c_cons_cons c t' cs \<Delta> ts' \<Gamma>)
+  thus ?case 
+  proof (cases x)
+    case 0
+    with tc\<^sub>c_cons_cons show ?thesis 
+    proof (cases y)
+      case (Suc y)
+      have "lookup (ts' # \<Gamma>) 0 = Some ts'" by simp
+      with tc\<^sub>c_cons_cons 0 Suc show ?thesis by fastforce
+    qed auto
+  next
+    case (Suc x)
+    with tc\<^sub>c_cons_cons Suc have "lookup (ts' # \<Gamma>) (Suc x) = Some ts" by simp
+    with tc\<^sub>c_cons_cons Suc show ?thesis by (cases y) fastforce+
+  qed
+qed simp_all
+
+lemma "c :\<^sub>g\<^sub>c\<^sub>l t \<Longrightarrow> True"
+  and tc_closure_mapfst [simp]: "\<Delta> :\<^sub>g\<^sub>c\<^sub>l\<^sub>s \<Gamma> \<Longrightarrow> c :\<^sub>g\<^sub>c\<^sub>l t \<Longrightarrow> 
+    mapfst ((#) c) \<Delta> :\<^sub>g\<^sub>c\<^sub>l\<^sub>s mapfst (insert_at 0 t) \<Gamma>"
+  by (induction c t and \<Delta> \<Gamma> rule: typing_closure\<^sub>g_typing_environment\<^sub>g.inducts) simp_all
+
+lemma canonical_num\<^sub>g [dest]: "c :\<^sub>g\<^sub>c\<^sub>l Num \<Longrightarrow> \<exists>n. c = Num\<^sub>g n"
+  by (induction c Num rule: typing_closure\<^sub>g_typing_environment\<^sub>g.inducts(1)) simp_all
+
+lemma canonical_arrow\<^sub>g [dest]: "c :\<^sub>g\<^sub>c\<^sub>l Arrow t\<^sub>1 t\<^sub>2 \<Longrightarrow> 
+    \<exists>\<Delta> \<Gamma> e. c = Fun\<^sub>g t\<^sub>1 \<Delta> e (let_count e) \<and> (\<Delta> :\<^sub>g\<^sub>c\<^sub>l\<^sub>s \<Gamma>) \<and> (insert_at 0 [t\<^sub>1] \<Gamma> \<turnstile>\<^sub>g e : t\<^sub>2)"
+  by (induction c "Arrow t\<^sub>1 t\<^sub>2" rule: typing_closure\<^sub>g_typing_environment\<^sub>g.inducts(1)) auto
+
+datatype frame\<^sub>g = 
+  FApp1\<^sub>g "closure\<^sub>g list list" expr\<^sub>g
+  | FApp2\<^sub>g closure\<^sub>g
+  | FLet\<^sub>g "closure\<^sub>g list list" expr\<^sub>g
+  | FPop\<^sub>g closure\<^sub>g
+  | FReturn\<^sub>g "closure\<^sub>g list list"
+
+fun latest_environment :: "frame\<^sub>g list \<rightharpoonup> closure\<^sub>g list list" where
+  "latest_environment [] = None"
+| "latest_environment (FApp1\<^sub>g \<Delta> e # s) = latest_environment s"
+| "latest_environment (FApp2\<^sub>g c # s) = latest_environment s"
+| "latest_environment (FLet\<^sub>g \<Delta> e # s) = latest_environment s"
+| "latest_environment (FPop\<^sub>g c # s) = map_option (mapfst ((#) c)) (latest_environment s)"
+| "latest_environment (FReturn\<^sub>g \<Delta> # s) = Some \<Delta>"
+
+inductive typing_stack\<^sub>g :: "frame\<^sub>g list \<Rightarrow> ty \<Rightarrow> ty \<Rightarrow> bool" (infix ":\<^sub>g _ \<rightarrow>" 50) where
+  tcc_snil [simp]: "[] :\<^sub>g t \<rightarrow> t"
+| tcc_scons_app1 [simp]: "\<Delta> :\<^sub>g\<^sub>c\<^sub>l\<^sub>s \<Gamma> \<Longrightarrow> \<Gamma> \<turnstile>\<^sub>g e : t\<^sub>1 \<Longrightarrow> s :\<^sub>g t\<^sub>2 \<rightarrow> t \<Longrightarrow> 
+    latest_environment s = Some \<Delta> \<Longrightarrow> FApp1\<^sub>g \<Delta> e # s :\<^sub>g Arrow t\<^sub>1 t\<^sub>2 \<rightarrow> t"
+| tcc_scons_app2 [simp]: "c :\<^sub>g\<^sub>c\<^sub>l Arrow t\<^sub>1 t\<^sub>2 \<Longrightarrow> s :\<^sub>g t\<^sub>2 \<rightarrow> t \<Longrightarrow> latest_environment s \<noteq> None \<Longrightarrow> 
+    FApp2\<^sub>g c # s :\<^sub>g t\<^sub>1 \<rightarrow> t"
+| tcc_scons_let [simp]: "latest_environment s = Some \<Delta> \<Longrightarrow> \<Delta> :\<^sub>g\<^sub>c\<^sub>l\<^sub>s \<Gamma> \<Longrightarrow> 
+    mapfst (insert_at 0 t\<^sub>1) \<Gamma> \<turnstile>\<^sub>g e : t\<^sub>2 \<Longrightarrow> s :\<^sub>g t\<^sub>2 \<rightarrow> t \<Longrightarrow> FLet\<^sub>g \<Delta> e # s :\<^sub>g t\<^sub>1 \<rightarrow> t"
+| tcc_scons_pop [simp]: "latest_environment s = Some \<Delta> \<Longrightarrow> c :\<^sub>g\<^sub>c\<^sub>l tt \<Longrightarrow> s :\<^sub>g t' \<rightarrow> t \<Longrightarrow> 
+    FPop\<^sub>g c # s :\<^sub>g t' \<rightarrow> t"
+| tcc_scons_ret [simp]: "\<Delta> :\<^sub>g\<^sub>c\<^sub>l\<^sub>s \<Gamma> \<Longrightarrow> s :\<^sub>g t' \<rightarrow> t \<Longrightarrow> FReturn\<^sub>g \<Delta> # s :\<^sub>g t' \<rightarrow> t"
+
+inductive_cases [elim]: "[] :\<^sub>g t' \<rightarrow> t"
+inductive_cases [elim]: "FApp1\<^sub>g \<Delta> e # s :\<^sub>g t' \<rightarrow> t"
+inductive_cases [elim]: "FApp2\<^sub>g c # s :\<^sub>g t' \<rightarrow> t"
+inductive_cases [elim]: "FLet\<^sub>g \<Delta> e # s :\<^sub>g t' \<rightarrow> t"
+inductive_cases [elim]: "FPop\<^sub>g c # s :\<^sub>g t' \<rightarrow> t"
+inductive_cases [elim]: "FReturn\<^sub>g \<Delta> # s :\<^sub>g t' \<rightarrow> t"
+
+datatype state\<^sub>g = 
+  SE\<^sub>g "frame\<^sub>g list" "closure\<^sub>g list list" expr\<^sub>g
+  | SC\<^sub>g "frame\<^sub>g list" closure\<^sub>g
+
+primrec final\<^sub>g :: "state\<^sub>g \<Rightarrow> bool" where
+  "final\<^sub>g (SE\<^sub>g s \<Delta> e) = False"
+| "final\<^sub>g (SC\<^sub>g s c) = (s = [])"
+
+inductive typecheck_state\<^sub>g :: "state\<^sub>g \<Rightarrow> ty \<Rightarrow> bool" (infix ":\<^sub>g" 50) where
+  tcc_state_ev [simp]: "s :\<^sub>g t' \<rightarrow> t \<Longrightarrow> \<Delta> :\<^sub>g\<^sub>c\<^sub>l\<^sub>s \<Gamma> \<Longrightarrow> latest_environment s = Some \<Delta> \<Longrightarrow> 
+    \<Gamma> \<turnstile>\<^sub>g e : t' \<Longrightarrow> SE\<^sub>g s \<Delta> e :\<^sub>g t"
+| tcc_state_ret [simp]: "s :\<^sub>g t' \<rightarrow> t \<Longrightarrow> c :\<^sub>g\<^sub>c\<^sub>l t' \<Longrightarrow> SC\<^sub>g s c :\<^sub>g t"
+
+inductive_cases [elim]: "SE\<^sub>g s \<Delta> e :\<^sub>g t"
+inductive_cases [elim]: "SC\<^sub>g s c :\<^sub>g t"
+
+text \<open>Evaluation, similarly, requires a slightly more complicated lookup than before, but is 
+otherwise unchanged.\<close>
+
+inductive eval\<^sub>g :: "state\<^sub>g \<Rightarrow> state\<^sub>g \<Rightarrow> bool" (infix "\<leadsto>\<^sub>g" 50) where
+  ev\<^sub>g_var [simp]: "lookup \<Delta> x = Some cs \<Longrightarrow> lookup cs y = Some c \<Longrightarrow> SE\<^sub>g s \<Delta> (Var\<^sub>g x y) \<leadsto>\<^sub>g SC\<^sub>g s c"
+| ev\<^sub>g_con [simp]: "SE\<^sub>g s \<Delta> (Const\<^sub>g n) \<leadsto>\<^sub>g SC\<^sub>g s (Num\<^sub>g n)"
+| ev\<^sub>g_lam [simp]: "SE\<^sub>g s \<Delta> (Lam\<^sub>g t e n) \<leadsto>\<^sub>g SC\<^sub>g s (Fun\<^sub>g t \<Delta> e n)"
+| ev\<^sub>g_app [simp]: "SE\<^sub>g s \<Delta> (App\<^sub>g e\<^sub>1 e\<^sub>2) \<leadsto>\<^sub>g SE\<^sub>g (FApp1\<^sub>g \<Delta> e\<^sub>2 # s) \<Delta> e\<^sub>1"
+| ev\<^sub>g_let [simp]: "SE\<^sub>g s \<Delta> (Let\<^sub>g e\<^sub>1 e\<^sub>2) \<leadsto>\<^sub>g SE\<^sub>g (FLet\<^sub>g \<Delta> e\<^sub>2 # s) \<Delta> e\<^sub>1"
+| ret\<^sub>g_app1 [simp]: "SC\<^sub>g (FApp1\<^sub>g \<Delta> e\<^sub>2 # s) c\<^sub>1 \<leadsto>\<^sub>g SE\<^sub>g (FApp2\<^sub>g c\<^sub>1 # s) \<Delta> e\<^sub>2"
+| ret\<^sub>g_app2 [simp]: "SC\<^sub>g (FApp2\<^sub>g (Fun\<^sub>g t \<Delta> e\<^sub>1 n) # s) c\<^sub>2 \<leadsto>\<^sub>g 
+    SE\<^sub>g (FReturn\<^sub>g ([c\<^sub>2] # \<Delta>) # s) ([c\<^sub>2] # \<Delta>) e\<^sub>1"
+| ret\<^sub>g_let [simp]: "SC\<^sub>g (FLet\<^sub>g \<Delta> e\<^sub>2 # s) c\<^sub>1 \<leadsto>\<^sub>g SE\<^sub>g (FPop\<^sub>g c\<^sub>1 # s) (mapfst ((#) c\<^sub>1) \<Delta>) e\<^sub>2"
+| ret\<^sub>g_pop [simp]: "SC\<^sub>g (FPop\<^sub>g c' # s) c \<leadsto>\<^sub>g SC\<^sub>g s c"
+| ret\<^sub>g_ret [simp]: "SC\<^sub>g (FReturn\<^sub>g \<Delta> # s) c \<leadsto>\<^sub>g SC\<^sub>g s c"
+
+text \<open>And the safety theorems:\<close>
+
+lemma eval\<^sub>g_from_nonvalue [simp]: "\<Gamma> \<turnstile>\<^sub>g e : t \<Longrightarrow> \<Delta> :\<^sub>g\<^sub>c\<^sub>l\<^sub>s \<Gamma> \<Longrightarrow> \<exists>\<Sigma>'. SE\<^sub>g s \<Delta> e \<leadsto>\<^sub>g \<Sigma>'"
+proof (induction \<Gamma> e t rule: typing\<^sub>g.induct)
+  case (tc\<^sub>g_var \<Gamma> x ts y t)
+  then obtain cs c where "lookup \<Delta> x = Some cs \<and> lookup cs y = Some c \<and> c :\<^sub>g\<^sub>c\<^sub>l t"
+    using lookup_in_env\<^sub>g by blast
+  hence "SE\<^sub>g s \<Delta> (Var\<^sub>g x y) \<leadsto>\<^sub>g SC\<^sub>g s c" by simp
+  thus ?case by fastforce 
+next
+  case (tc\<^sub>g_const \<Gamma> n)
+  have "SE\<^sub>g s \<Delta> (Const\<^sub>g n) \<leadsto>\<^sub>g SC\<^sub>g s (Num\<^sub>g n)" by simp
+  thus ?case by fastforce 
+next
+  case (tc\<^sub>g_lam t\<^sub>1 \<Gamma> e t\<^sub>2)
+  have "SE\<^sub>g s \<Delta> (Lam\<^sub>g t\<^sub>1 e (let_count e)) \<leadsto>\<^sub>g SC\<^sub>g s (Fun\<^sub>g t\<^sub>1 \<Delta> e (let_count e))" by simp
+  thus ?case by fastforce 
+next
+  case (tc\<^sub>g_app \<Gamma> e\<^sub>1 t\<^sub>1 t\<^sub>2 e\<^sub>2)
+  have "SE\<^sub>g s \<Delta> (App\<^sub>g e\<^sub>1 e\<^sub>2) \<leadsto>\<^sub>g SE\<^sub>g (FApp1\<^sub>g \<Delta> e\<^sub>2 # s) \<Delta> e\<^sub>1" by simp
+  thus ?case by fastforce
+next
+  case (tc\<^sub>g_let \<Gamma> e\<^sub>1 t\<^sub>1 e\<^sub>2 t\<^sub>2)
+  have "SE\<^sub>g s \<Delta> (Let\<^sub>g e\<^sub>1 e\<^sub>2) \<leadsto>\<^sub>g SE\<^sub>g (FLet\<^sub>g \<Delta> e\<^sub>2 # s) \<Delta> e\<^sub>1" by simp
+  thus ?case by fastforce
+qed
+
+lemma eval\<^sub>g_from_value [simp]: "s :\<^sub>g t' \<rightarrow> t \<Longrightarrow> c :\<^sub>g\<^sub>c\<^sub>l t' \<Longrightarrow> s = [] \<or> (\<exists>\<Sigma>'. SC\<^sub>g s c \<leadsto>\<^sub>g \<Sigma>')"
+proof (induction s t' t rule: typing_stack\<^sub>g.induct)
+  case (tcc_scons_app1 \<Delta> \<Gamma> e\<^sub>2 t\<^sub>1 s t\<^sub>2 t)
+  moreover hence "SC\<^sub>g (FApp1\<^sub>g \<Delta> e\<^sub>2 # s) c \<leadsto>\<^sub>g SE\<^sub>g (FApp2\<^sub>g c # s) \<Delta> e\<^sub>2" by simp
+  ultimately show ?case by fastforce
+next
+  case (tcc_scons_app2 c\<^sub>1 t\<^sub>1 t\<^sub>2 s t)
+  then obtain \<Delta> ts e where "c\<^sub>1 = Fun\<^sub>g t\<^sub>1 \<Delta> e (let_count e) \<and> (\<Delta> :\<^sub>g\<^sub>c\<^sub>l\<^sub>s ts) \<and> 
+    (insert_at 0 [t\<^sub>1] ts \<turnstile>\<^sub>g e : t\<^sub>2)" by blast
+  moreover hence "SC\<^sub>g (FApp2\<^sub>g (Fun\<^sub>g t\<^sub>1 \<Delta> e (let_count e)) # s) c \<leadsto>\<^sub>g 
+    SE\<^sub>g (FReturn\<^sub>g ([c] # \<Delta>) # s) ([c] # \<Delta>) e" by simp
+  ultimately show ?case by fastforce
+next
+  case (tcc_scons_let s \<Delta> \<Gamma> t\<^sub>1 e t\<^sub>2 t)
+  have "SC\<^sub>g (FLet\<^sub>g \<Delta> e # s) c \<leadsto>\<^sub>g SE\<^sub>g (FPop\<^sub>g c # s) (mapfst ((#) c) \<Delta>) e" by simp
+  thus ?case by fastforce
+next
+  case (tcc_scons_pop s \<Delta> c' \<Gamma> t' t)
+  have "SC\<^sub>g (FPop\<^sub>g c' # s) c \<leadsto>\<^sub>g SC\<^sub>g s c" by simp
+  thus ?case by fastforce
+next
+  case (tcc_scons_ret \<Delta> \<Gamma> s t' t)
+  have "SC\<^sub>g (FReturn\<^sub>g \<Delta> # s) c \<leadsto>\<^sub>g SC\<^sub>g s c" by simp
+  thus ?case by fastforce
+qed simp_all
+
+theorem progress\<^sub>g: "\<Sigma> :\<^sub>g t \<Longrightarrow> final\<^sub>g \<Sigma> \<or> (\<exists>\<Sigma>'. \<Sigma> \<leadsto>\<^sub>g \<Sigma>')"
+  by (induction \<Sigma> t rule: typecheck_state\<^sub>g.induct) simp_all
+
+lemma final_no_eval\<^sub>g [simp]: "\<Sigma> \<leadsto>\<^sub>g \<Sigma>' \<Longrightarrow> final\<^sub>g \<Sigma> \<Longrightarrow> False"
+  by (induction \<Sigma> \<Sigma>' rule: eval\<^sub>g.induct) simp_all
+
+theorem preservation\<^sub>g [simp]: "\<Sigma> \<leadsto>\<^sub>g \<Sigma>' \<Longrightarrow> \<Sigma> :\<^sub>g t \<Longrightarrow> \<Sigma>' :\<^sub>g t"
+proof (induction \<Sigma> \<Sigma>' rule: eval\<^sub>g.induct)
+  case (ev\<^sub>g_var \<Delta> x cs y c s)
+  then obtain ts t' \<Gamma> where X: "s :\<^sub>g t' \<rightarrow> t" and "(\<Delta> :\<^sub>g\<^sub>c\<^sub>l\<^sub>s \<Gamma>) \<and> lookup \<Gamma> x = Some ts \<and> 
+    lookup ts y = Some t'" by blast
+  then obtain cs c' where "lookup \<Delta> x = Some cs \<and> lookup cs y = Some c' \<and> c' :\<^sub>g\<^sub>c\<^sub>l t'"
+    using lookup_in_env\<^sub>g by blast
+  with ev\<^sub>g_var X show ?case by simp
+next
+  case (ev\<^sub>g_app s \<Delta> e\<^sub>1 e\<^sub>2)
+  then obtain t\<^sub>1 t\<^sub>2 \<Gamma> where "(s :\<^sub>g t\<^sub>2 \<rightarrow> t) \<and> (\<Gamma> \<turnstile>\<^sub>g e\<^sub>2 : t\<^sub>1)" 
+   and X: "(\<Delta> :\<^sub>g\<^sub>c\<^sub>l\<^sub>s \<Gamma>) \<and> latest_environment s = Some \<Delta> \<and> (\<Gamma> \<turnstile>\<^sub>g e\<^sub>1 : Arrow t\<^sub>1 t\<^sub>2)" by blast
+  hence "FApp1\<^sub>g \<Delta> e\<^sub>2 # s :\<^sub>g Arrow t\<^sub>1 t\<^sub>2 \<rightarrow> t"  by fastforce
+  with X show ?case by fastforce
+next
+  case (ev\<^sub>g_let s \<Delta> e\<^sub>1 e\<^sub>2)
+  then obtain \<Gamma> t\<^sub>2 t\<^sub>1 where "(s :\<^sub>g t\<^sub>2 \<rightarrow> t) \<and> (mapfst (insert_at 0 t\<^sub>1) \<Gamma> \<turnstile>\<^sub>g e\<^sub>2 : t\<^sub>2)" 
+    and X: "(\<Gamma> \<turnstile>\<^sub>g e\<^sub>1 : t\<^sub>1) \<and> (\<Delta> :\<^sub>g\<^sub>c\<^sub>l\<^sub>s \<Gamma>) \<and> latest_environment s = Some \<Delta>" by fastforce
+  hence "FLet\<^sub>g \<Delta> e\<^sub>2 # s :\<^sub>g t\<^sub>1 \<rightarrow> t" by fastforce
+  with X show ?case by fastforce
+next
+  case (ret\<^sub>g_app1 \<Delta> e\<^sub>2 s c\<^sub>1)
+  then obtain \<Gamma> t\<^sub>1 t\<^sub>2 where X: "(\<Delta> :\<^sub>g\<^sub>c\<^sub>l\<^sub>s \<Gamma>) \<and> latest_environment s = Some \<Delta> \<and> (\<Gamma> \<turnstile>\<^sub>g e\<^sub>2 : t\<^sub>1)" 
+   and "(s :\<^sub>g t\<^sub>2 \<rightarrow> t) \<and> (c\<^sub>1 :\<^sub>g\<^sub>c\<^sub>l Arrow t\<^sub>1 t\<^sub>2)" by blast
+  hence "FApp2\<^sub>g c\<^sub>1 # s :\<^sub>g t\<^sub>1 \<rightarrow> t" by fastforce
+  with X show ?case by fastforce
+next
+  case (ret\<^sub>g_app2 t\<^sub>1 \<Delta> e\<^sub>1 n s c\<^sub>2)
+  then obtain \<Gamma> t\<^sub>2 where X: "s :\<^sub>g t\<^sub>2 \<rightarrow> t" and Y: "insert_at 0 [t\<^sub>1] \<Gamma> \<turnstile>\<^sub>g e\<^sub>1 : t\<^sub>2" 
+   and "(\<Delta> :\<^sub>g\<^sub>c\<^sub>l\<^sub>s \<Gamma>) \<and> (c\<^sub>2 :\<^sub>g\<^sub>c\<^sub>l t\<^sub>1)" by blast
+  hence Z: "[c\<^sub>2] # \<Delta> :\<^sub>g\<^sub>c\<^sub>l\<^sub>s insert_at 0 [t\<^sub>1] \<Gamma>" by (cases \<Gamma>) simp_all
+  with X have "FReturn\<^sub>g ([c\<^sub>2] # \<Delta>) # s :\<^sub>g t\<^sub>2 \<rightarrow> t" by simp
+  with Y Z show ?case by fastforce
+next
+  case (ret\<^sub>g_let \<Delta> e\<^sub>2 s c\<^sub>1)
+  then obtain \<Gamma> t\<^sub>1 t\<^sub>2 where X: "mapfst (insert_at 0 t\<^sub>1) \<Gamma> \<turnstile>\<^sub>g e\<^sub>2 : t\<^sub>2" and "\<Delta> :\<^sub>g\<^sub>c\<^sub>l\<^sub>s \<Gamma>" 
+    and A: "c\<^sub>1 :\<^sub>g\<^sub>c\<^sub>l t\<^sub>1" and Y: "s :\<^sub>g t\<^sub>2 \<rightarrow> t" and Z: "latest_environment s = Some \<Delta>" by fastforce
+  hence W: "mapfst ((#) c\<^sub>1) \<Delta> :\<^sub>g\<^sub>c\<^sub>l\<^sub>s mapfst (insert_at 0 t\<^sub>1) \<Gamma>" by simp
+  from Y Z A have "FPop\<^sub>g c\<^sub>1 # s :\<^sub>g t\<^sub>2 \<rightarrow> t" by simp
+  with X Z W show ?case by fastforce
+qed fastforce+
+
+lemma preservation\<^sub>g_iter [simp]: "iter (\<leadsto>\<^sub>g) \<Sigma> \<Sigma>' \<Longrightarrow> \<Sigma> :\<^sub>g t \<Longrightarrow> \<Sigma>' :\<^sub>g t"
+  by (induction \<Sigma> \<Sigma>' rule: iter.induct) simp_all
+
+theorem determinism\<^sub>g: "\<Sigma> \<leadsto>\<^sub>g \<Sigma>' \<Longrightarrow> \<Sigma> \<leadsto>\<^sub>g \<Sigma>'' \<Longrightarrow> \<Sigma>' = \<Sigma>''"
+proof (induction \<Sigma> \<Sigma>' rule: eval\<^sub>g.induct)
+  case (ev\<^sub>g_var \<Delta> x c s)
+  from ev\<^sub>g_var(3, 1, 2) show ?case by (induction rule: eval\<^sub>g.cases) simp_all 
+next
+  case (ev\<^sub>g_con s \<Delta> k)
+  thus ?case by (induction rule: eval\<^sub>g.cases) simp_all 
+next
+  case (ev\<^sub>g_lam s \<Delta> t e)
+  thus ?case by (induction rule: eval\<^sub>g.cases) simp_all 
+next
+  case (ev\<^sub>g_app s \<Delta> e\<^sub>1 e\<^sub>2)
+  thus ?case by (induction rule: eval\<^sub>g.cases) simp_all 
+next
+  case (ev\<^sub>g_let s \<Delta> e\<^sub>1 e\<^sub>2)
+  thus ?case by (induction rule: eval\<^sub>g.cases) simp_all 
+next
+  case (ret\<^sub>g_app1 \<Delta> e\<^sub>2 s c\<^sub>1)
+  thus ?case by (induction rule: eval\<^sub>g.cases) simp_all 
+next
+  case (ret\<^sub>g_app2 t \<Delta> e\<^sub>1 s c\<^sub>2)
+  thus ?case by (induction rule: eval\<^sub>g.cases) simp_all 
+next
+  case (ret\<^sub>g_let \<Delta> e\<^sub>2 s c\<^sub>1)
+  thus ?case by (induction rule: eval\<^sub>g.cases) simp_all 
+next
+  case (ret\<^sub>g_pop s c)
+  thus ?case by (induction rule: eval\<^sub>g.cases) simp_all 
+next
+  case (ret\<^sub>g_ret \<Delta> s c)
+  thus ?case by (induction rule: eval\<^sub>g.cases) simp_all 
+qed
+
+end
